crypto_examples/mulntt_ct/mulntt_ct_rec.dfy
@@ -13,14 +13,21 @@ module mulntt_ct_rec {
 
     import opened nth_root
     import opened ntt_index
+    import opened ntt_polys
 
     function method A(): seq<elem>
         ensures |A()| == N == pow2(LOGN).full;
 
-    function method block_count(m: pow2_t): nat
+    function method block_count(m: pow2_t): pow2_t
         requires 0 <= m.exp <= LOGN;
     {
-        pow2_div(pow2(LOGN), m).full
+        pow2_div(pow2(LOGN), m)
+    }
+
+    function method block_size(c: pow2_t): pow2_t
+        requires 0 <= c.exp <= LOGN;
+    {
+        pow2_div(pow2(LOGN), c)
     }
 
     // lemma block_count_product_lemma(m: pow2_t)
@@ -32,7 +39,7 @@ module mulntt_ct_rec {
 
     lemma block_count_half_lemma(m: pow2_t)
         requires 1 <= m.exp <= LOGN;
-        ensures block_count(pow2_half(m)) == block_count(m) * 2;
+        ensures block_count(pow2_half(m)) == pow2_double(block_count(m));
     {
         Nth_root_lemma();
         var left := pow2_div(pow2(LOGN), pow2_half(m));
@@ -53,16 +60,26 @@ module mulntt_ct_rec {
         LemmaMulEqualityConverse(half, left.full, right.full * 2);
     }
 
+    predicate {:opaque} unifromly_sized(blocks: seq<seq<elem>>, bsize: pow2_t)
+        requires bsize.exp <= LOGN;
+        ensures unifromly_sized(blocks, bsize)
+            ==> |blocks| == block_count(bsize).full;
+    {
+        && (forall i: nat | i < |blocks| :: |blocks[i]| == bsize.full)
+        && |blocks| == block_count(bsize).full
+    }
+
+
     type n_sized = s: seq<elem>
         | |s| == N == pow2(LOGN).full witness *
     
     lemma point_view_index_bound_lemma(i: nat, j: nat, bsize: pow2_t)
         requires bsize.exp <= LOGN;
-        requires i < block_count(bsize);
+        requires i < block_count(bsize).full;
         requires j < bsize.full;
-        ensures 0 <= i + j * block_count(bsize) < N;
+        ensures 0 <= i + j * block_count(bsize).full < N;
     {
-        var count := block_count(bsize);
+        var count := block_count(bsize).full;
         calc {
             i + j * count;
             <=
@@ -81,17 +98,17 @@ module mulntt_ct_rec {
 
     function point_view_index(i: nat, j: nat, bsize: pow2_t): (offset: nat)
         requires bsize.exp <= LOGN;
-        requires i < block_count(bsize);
+        requires i < block_count(bsize).full;
         requires j < bsize.full;
         ensures offset < N;
     {
         point_view_index_bound_lemma(i, j, bsize);
-        i + j * block_count(bsize)
+        i + j * block_count(bsize).full
     }
 
     function points_view(a: n_sized, i: nat, bsize: pow2_t): (v: seq<elem>)
         requires bsize.exp <= LOGN;
-        requires i < block_count(bsize);
+        requires i < block_count(bsize).full;
         // ensures |v| == bsize.full;
     {
         var size := bsize.full;
@@ -104,7 +121,7 @@ module mulntt_ct_rec {
         requires bsize.exp <= LOGN;
         ensures unifromly_sized(vs, bsize);
     {
-        var count := block_count(bsize);
+        var count := block_count(bsize).full;
         var vs := seq(count, i requires 0 <= i < count => points_view(a, i, bsize));
         assert unifromly_sized(vs, bsize) by {
             reveal unifromly_sized();
@@ -167,4 +184,211 @@ module mulntt_ct_rec {
         reveal unifromly_sized();
         reveal build_lower_level();
     }
+
+    function bit_rev_int(i: nat, bound: pow2_t): (j: nat)
+        requires i < bound.full;
+        ensures j < bound.full;
+
+    // d is the block count
+    function x_value(i: nat, d: pow2_t): elem
+        requires d.exp <= LOGN;
+        requires i < block_size(d).full;
+    {
+        var bound := pow2_div(pow2(LOGN), d);
+        LemmaMulNonnegative(d.full, bit_rev_int(i, bound));
+        modmul(modpow(OMEGA, d.full * bit_rev_int(i, bound)), modpow(PSI, d.full))
+    }
+
+    // d is the block count
+    predicate {:opaque} points_eval_prefix_inv(points: seq<elem>, poly: seq<elem>, l: nat, d: pow2_t)
+    {
+        && d.exp <= LOGN
+        && l <= |points| == |poly| == block_size(d).full
+        && forall i | 0 <= i < l :: poly_eval(poly, x_value(i, d)) == points[i]
+    }
+
+    // d is the block count
+    predicate {:opaque} points_eval_suffix_inv(points: seq<elem>, poly: seq<elem>, l: nat, d: pow2_t)
+    {
+        && d.exp <= LOGN
+        && l <= |points| == |poly| == block_size(d).full
+        && forall i | l <= i < block_size(d).full ::
+            poly_eval(poly, x_value(i, d)) == points[i]
+    }
+
+    datatype s_loop_view = s_loop_view(
+        lower: seq<seq<elem>>, // lower polys
+        higher: seq<seq<elem>>, // higher polys
+        hsize: pow2_t)
+    {
+        predicate s_loop_wf()
+        {
+            && 1 <= hsize.exp <= LOGN
+            && unifromly_sized(higher, hsize)
+            && build_lower_level(higher, hsize) == lower
+        }
+
+        function lsize(): pow2_t
+            requires s_loop_wf();
+        {
+            pow2_half(hsize)
+        }
+
+        function lcount(): pow2_t
+            requires s_loop_wf();
+        {
+            block_count(lsize())
+        }
+
+        function hcount(): pow2_t
+            requires s_loop_wf();
+        {
+            block_count(hsize)
+        }
+
+        lemma size_count_lemma()
+            requires s_loop_wf();
+            ensures pow2_double(lsize()) == hsize;
+            ensures lcount() == pow2_double(hcount());
+            ensures lcount().full * lsize().full
+                == hcount().full * hsize.full == N;
+        {
+            Nth_root_lemma();
+            block_count_half_lemma(hsize);
+        }
+
+        predicate {:opaque} s_loop_higher_inv(a: n_sized, hcount: pow2_t, j: nat, bi: nat)
+            requires hcount.exp <= LOGN;
+            requires bi < hcount.full;
+            requires s_loop_wf();
+            requires hsize == block_size(hcount);
+        {
+            && var hpoints := level_points_view(a, hsize);
+            && (forall i | 0 <= i < bi ::
+                points_eval_prefix_inv(hpoints[i], higher[bit_rev_int(i, hcount)], 2*j+2, hcount))
+            && (forall i | bi <= i < hcount.full ::
+                points_eval_prefix_inv(hpoints[i], higher[bit_rev_int(i, hcount)], 2*j, hcount))
+        }
+
+        predicate {:opaque} s_loop_lower_inv(a: n_sized, hcount: pow2_t, j: nat, bi: nat)
+            requires hcount.exp <= LOGN;
+            requires bi < hcount.full;
+            requires s_loop_wf();
+            requires hsize == block_size(hcount);
+        {
+            size_count_lemma();
+            && var lcount := lcount();
+            && var lpoints := level_points_view(a, lsize());
+            && (forall i | (0 <= i < bi || hcount.full <= i < bi + hcount.full) ::
+                && (points_eval_suffix_inv(lpoints[i], lower[bit_rev_int(i, lcount)], j+1, lcount)))
+            && (forall i | (bi <= i < hcount.full || bi + hcount.full <= i < lcount.full) ::
+                points_eval_suffix_inv(lpoints[i], lower[bit_rev_int(i, lcount)], j, lcount))
+        }
+
+        predicate s_loop_inv(a: n_sized, hcount: pow2_t, j: nat, bi: nat)
+        {
+            && s_loop_wf()
+            && hcount.exp <= LOGN
+            && bi < hcount.full
+            && j < lsize().full
+            && hsize == block_size(hcount)
+            && s_loop_higher_inv(a, hcount, j, bi)
+            && s_loop_lower_inv(a, hcount, j, bi)
+        }
+
+        lemma higher_points_view_index_lemma(a: n_sized, hcount: pow2_t, j: nat, bi: nat, s: nat)
+            requires s_loop_inv(a, hcount, j, bi);
+            requires s == bi + (2*j) * hcount.full;
+            ensures s + hcount.full < N;
+            ensures a[s] == level_points_view(a, hsize)[bi][2*j];
+            ensures a[s+hcount.full] == level_points_view(a, hsize)[bi][2*j+1];
+        {
+            size_count_lemma();
+            var hpoints := level_points_view(a, hsize);
+
+            calc == {
+                hpoints[bi][2*j];
+                points_view(a, bi, hsize)[2*j];
+                a[point_view_index(bi, 2*j, hsize)];
+                {
+                    assert s == point_view_index(bi, 2*j, hsize);
+                }
+                a[s];
+            }
+
+            calc == {
+                s + hcount.full;
+                point_view_index(bi, 2*j, hsize) + hcount.full;
+                bi + (2*j) * hcount.full + hcount.full;
+                {
+                    LemmaMulIsDistributiveAddOtherWayAuto();
+                }
+                bi + (2*j+1) * hcount.full;
+                point_view_index(bi, 2*j+1, hsize);
+            }
+
+            calc == {
+                hpoints[bi][2*j+1];
+                points_view(a, bi, hsize)[2*j+1];
+                a[point_view_index(bi, 2*j+1, hsize)];
+                a[s + hcount.full];
+            }
+        }
+
+        lemma lower_points_view_index_lemma(a: n_sized, hcount: pow2_t, j: nat, bi: nat, s: nat)
+            requires s_loop_inv(a, hcount, j, bi);
+            requires s == bi + (2*j) * hcount.full;
+            ensures s + hcount.full < N;
+            ensures bi + hcount.full < lcount().full;
+            ensures a[s] == level_points_view(a, lsize())[bi][j];
+            ensures a[s+hcount.full] == level_points_view(a, lsize())[bi+hcount.full][j];
+        {
+            size_count_lemma();
+            var lpoints := level_points_view(a, lsize());
+
+            calc == {
+                s;
+                bi + (2*j) * hcount.full;
+                {
+                    LemmaMulIsAssociativeAuto();
+                }
+                bi + j * (2*hcount.full);
+                point_view_index(bi, j, lsize());
+            }
+
+            calc == {
+                lpoints[bi][j];
+                points_view(a, bi, lsize())[j];
+                a[point_view_index(bi, j, lsize())];
+                a[s];
+            }
+
+            calc == {
+                s + hcount.full;
+                bi + hcount.full + (j*2) * hcount.full;
+                {
+                    LemmaMulIsAssociativeAuto();
+                }
+                bi + hcount.full + j * (2 * hcount.full);
+                bi + hcount.full + j * lcount().full;
+                point_view_index(bi +  hcount.full, j, lsize());
+            }
+
+            calc == {
+                lpoints[bi+hcount.full][j];
+                points_view(a, bi+hcount.full, lsize())[j];
+                a[point_view_index(bi+hcount.full, j, lsize())];
+                a[s+hcount.full];
+            }
+        }
+
+        // lemma s_loop_inv_preserved(a: n_sized, a': n_sized, hcount: pow2_t, j: nat, bi: nat)
+        //     requires s_loop_inv(a, hcount, j, bi);
+        // {
+
+
+        // }
+    }
+    // function level_points_view(a: n_sized, bsize: pow2_t): (vs: seq<seq<elem>>)
+
 }
